parametrizing gemms by their size requirement

src/lib/inst/gemm/Kuiper.GEMM.BlockTiling1D.fsti
@@ -10,53 +10,61 @@ open Kuiper.Matrix.Reprs { row_major as RM, col_major as CM }
    stack-allocated variable-length array, and NVCC complains
    (karamel warns too). *)
 
+// Pretty hideous. But this must match the pure resource in the precondition of
+// the kernel exactly. Should we make it a squashed argument instead, to take
+// advantage of subtyping?
+let size_req tile : size_req_t =
+  fun rows shared cols ->
+    (rows / tile) * (cols / tile) <= max_blocks /\
+    tile * tile <= max_threads
+
 (* Specialized to tile=32 *)
 
-val matmul_f32_tile32_rrr : fixed_repr_matmul_cpu_ty f32 RM RM RM
-val matmul_f64_tile32_rrr : fixed_repr_matmul_cpu_ty f64 RM RM RM
-val matmul_u32_tile32_rrr : fixed_repr_matmul_cpu_ty u32 RM RM RM
-val matmul_u64_tile32_rrr : fixed_repr_matmul_cpu_ty u64 RM RM RM
+val matmul_f32_tile32_rrr : fixed_repr_matmul_cpu_ty f32 (size_req 32) RM RM RM
+val matmul_f64_tile32_rrr : fixed_repr_matmul_cpu_ty f64 (size_req 32) RM RM RM
+val matmul_u32_tile32_rrr : fixed_repr_matmul_cpu_ty u32 (size_req 32) RM RM RM
+val matmul_u64_tile32_rrr : fixed_repr_matmul_cpu_ty u64 (size_req 32) RM RM RM
 
-val matmul_f32_tile32_ccc : fixed_repr_matmul_cpu_ty f32 CM CM CM
-val matmul_f64_tile32_ccc : fixed_repr_matmul_cpu_ty f64 CM CM CM
-val matmul_u32_tile32_ccc : fixed_repr_matmul_cpu_ty u32 CM CM CM
-val matmul_u64_tile32_ccc : fixed_repr_matmul_cpu_ty u64 CM CM CM
+val matmul_f32_tile32_ccc : fixed_repr_matmul_cpu_ty f32 (size_req 32) CM CM CM
+val matmul_f64_tile32_ccc : fixed_repr_matmul_cpu_ty f64 (size_req 32) CM CM CM
+val matmul_u32_tile32_ccc : fixed_repr_matmul_cpu_ty u32 (size_req 32) CM CM CM
+val matmul_u64_tile32_ccc : fixed_repr_matmul_cpu_ty u64 (size_req 32) CM CM CM
 
 (* Specialized to tile=16 *)
 
-val matmul_f32_tile16_rrr : fixed_repr_matmul_cpu_ty f32 RM RM RM
-val matmul_f64_tile16_rrr : fixed_repr_matmul_cpu_ty f64 RM RM RM
-val matmul_u32_tile16_rrr : fixed_repr_matmul_cpu_ty u32 RM RM RM
-val matmul_u64_tile16_rrr : fixed_repr_matmul_cpu_ty u64 RM RM RM
+val matmul_f32_tile16_rrr : fixed_repr_matmul_cpu_ty f32 (size_req 16) RM RM RM
+val matmul_f64_tile16_rrr : fixed_repr_matmul_cpu_ty f64 (size_req 16) RM RM RM
+val matmul_u32_tile16_rrr : fixed_repr_matmul_cpu_ty u32 (size_req 16) RM RM RM
+val matmul_u64_tile16_rrr : fixed_repr_matmul_cpu_ty u64 (size_req 16) RM RM RM
 
-val matmul_f32_tile16_ccc : fixed_repr_matmul_cpu_ty f32 CM CM CM
-val matmul_f64_tile16_ccc : fixed_repr_matmul_cpu_ty f64 CM CM CM
-val matmul_u32_tile16_ccc : fixed_repr_matmul_cpu_ty u32 CM CM CM
-val matmul_u64_tile16_ccc : fixed_repr_matmul_cpu_ty u64 CM CM CM
+val matmul_f32_tile16_ccc : fixed_repr_matmul_cpu_ty f32 (size_req 16) CM CM CM
+val matmul_f64_tile16_ccc : fixed_repr_matmul_cpu_ty f64 (size_req 16) CM CM CM
+val matmul_u32_tile16_ccc : fixed_repr_matmul_cpu_ty u32 (size_req 16) CM CM CM
+val matmul_u64_tile16_ccc : fixed_repr_matmul_cpu_ty u64 (size_req 16) CM CM CM
 
 
 (* Below are GPU-side versions: they take live GPU pointers and do not memcpy. *)
 
 (* Specialized to tile=32 *)
 
-val g_matmul_f32_tile32_rrr : fixed_repr_mmcomb_gpu_ty f32 RM RM RM
-val g_matmul_f64_tile32_rrr : fixed_repr_mmcomb_gpu_ty f64 RM RM RM
-val g_matmul_u32_tile32_rrr : fixed_repr_mmcomb_gpu_ty u32 RM RM RM
-val g_matmul_u64_tile32_rrr : fixed_repr_mmcomb_gpu_ty u64 RM RM RM
+val g_matmul_f32_tile32_rrr : fixed_repr_mmcomb_gpu_ty f32 (size_req 32) RM RM RM
+val g_matmul_f64_tile32_rrr : fixed_repr_mmcomb_gpu_ty f64 (size_req 32) RM RM RM
+val g_matmul_u32_tile32_rrr : fixed_repr_mmcomb_gpu_ty u32 (size_req 32) RM RM RM
+val g_matmul_u64_tile32_rrr : fixed_repr_mmcomb_gpu_ty u64 (size_req 32) RM RM RM
 
-val g_matmul_f32_tile32_ccc : fixed_repr_mmcomb_gpu_ty f32 CM CM CM
-val g_matmul_f64_tile32_ccc : fixed_repr_mmcomb_gpu_ty f64 CM CM CM
-val g_matmul_u32_tile32_ccc : fixed_repr_mmcomb_gpu_ty u32 CM CM CM
-val g_matmul_u64_tile32_ccc : fixed_repr_mmcomb_gpu_ty u64 CM CM CM
+val g_matmul_f32_tile32_ccc : fixed_repr_mmcomb_gpu_ty f32 (size_req 32) CM CM CM
+val g_matmul_f64_tile32_ccc : fixed_repr_mmcomb_gpu_ty f64 (size_req 32) CM CM CM
+val g_matmul_u32_tile32_ccc : fixed_repr_mmcomb_gpu_ty u32 (size_req 32) CM CM CM
+val g_matmul_u64_tile32_ccc : fixed_repr_mmcomb_gpu_ty u64 (size_req 32) CM CM CM
 
 (* Specialized to tile=16 *)
 
-val g_matmul_f32_tile16_rrr : fixed_repr_mmcomb_gpu_ty f32 RM RM RM
-val g_matmul_f64_tile16_rrr : fixed_repr_mmcomb_gpu_ty f64 RM RM RM
-val g_matmul_u32_tile16_rrr : fixed_repr_mmcomb_gpu_ty u32 RM RM RM
-val g_matmul_u64_tile16_rrr : fixed_repr_mmcomb_gpu_ty u64 RM RM RM
+val g_matmul_f32_tile16_rrr : fixed_repr_mmcomb_gpu_ty f32 (size_req 16) RM RM RM
+val g_matmul_f64_tile16_rrr : fixed_repr_mmcomb_gpu_ty f64 (size_req 16) RM RM RM
+val g_matmul_u32_tile16_rrr : fixed_repr_mmcomb_gpu_ty u32 (size_req 16) RM RM RM
+val g_matmul_u64_tile16_rrr : fixed_repr_mmcomb_gpu_ty u64 (size_req 16) RM RM RM
 
-val g_matmul_f32_tile16_ccc : fixed_repr_mmcomb_gpu_ty f32 CM CM CM
-val g_matmul_f64_tile16_ccc : fixed_repr_mmcomb_gpu_ty f64 CM CM CM
-val g_matmul_u32_tile16_ccc : fixed_repr_mmcomb_gpu_ty u32 CM CM CM
-val g_matmul_u64_tile16_ccc : fixed_repr_mmcomb_gpu_ty u64 CM CM CM
+val g_matmul_f32_tile16_ccc : fixed_repr_mmcomb_gpu_ty f32 (size_req 16) CM CM CM
+val g_matmul_f64_tile16_ccc : fixed_repr_mmcomb_gpu_ty f64 (size_req 16) CM CM CM
+val g_matmul_u32_tile16_ccc : fixed_repr_mmcomb_gpu_ty u32 (size_req 16) CM CM CM
+val g_matmul_u64_tile16_ccc : fixed_repr_mmcomb_gpu_ty u64 (size_req 16) CM CM CM
