src/lib/inst/gemm/Kuiper.GEMM.OrigBlockTiling1D.fsti
@@ -9,7 +9,11 @@ open Kuiper.Matrix.Reprs { row_major as RM, col_major as CM }
    stack-allocated variable-length array, and NVCC complains
    (karamel warns too). *)
 
-val matmul_f32_tiles64x8_8x64_rc8_rrr : fixed_repr_matmul_cpu_ty f32 RM RM RM
+let size_req tile : size_req_t =
+  fun rows shared cols ->
+    (rows / tile) * (cols / tile) <= max_blocks
+
+val matmul_f32_tiles64x8_8x64_rc8_rrr : fixed_repr_matmul_cpu_ty f32 (size_req 64) RM RM RM
 // This combination of tile sizes is forbidden!
 //  The generated code contains dynamic guards that immediately fail.
-// val matmul_f32_tiles32x32_32x32_rc32_rrr : fixed_repr_matmul_cpu_ty f32 RM RM RM
+// val matmul_f32_tiles32x32_32x32_rc32_rrr : fixed_repr_matmul_cpu_ty f32 (size_req 32) RM RM RM
