src/lib/poly/gemm/Kuiper.Poly.GEMM.Naive.fst
@@ -293,7 +293,7 @@ fn mmcomb_gpu
     gA |-> Frac fA eA **
     gB |-> Frac fB eB
   requires
-    pure (rows * cols <= max_blocks) **
+    pure (rows * cols <= max_blocks) ** (* size_req *)
     gC |-> eC
   ensures
     gC |-> MS.mmcomb comb eC eA eB
