src/lib/poly/gemm/Kuiper.Poly.GEMM.Tiled.fsti
@@ -5,5 +5,10 @@ module Kuiper.Poly.GEMM.Tiled
 open Kuiper
 open Kuiper.Poly.GEMMGPU.Type
 
+let size_req : tiled_size_req_t =
+  fun mrows mshared mcols tile ->
+    mrows * mcols <= max_blocks /\
+    tile * tile <= max_threads
+
 inline_for_extraction noextract
-val mmcomb_gpu : tiled_matmulcomb_gpu_ty
+val mmcomb_gpu : tiled_matmulcomb_gpu_ty size_req
