src/lib/poly/gemm/Kuiper.Poly.GEMMGPU.Type.fsti
@@ -14,6 +14,12 @@ module M4 = Kuiper.Matrix4
    we're working with. For now, just use this definition. *)
 type valid_tile = tile:szp{tile * tile <= max_threads}
 
+(* Maybe make this szp -> szp -> szp -> bool? *)
+inline_for_extraction noextract
+type size_req_t = nat -> nat -> nat -> prop
+inline_for_extraction noextract
+type tiled_size_req_t = nat -> nat -> nat -> nat ->prop
+
 unfold
 inline_for_extraction
 type matmulcomb_gpu_fixed_ty
@@ -25,6 +31,7 @@ type matmulcomb_gpu_fixed_ty
   (lA : full_mlayout rows shared)
   (lB : full_mlayout shared cols)
   (lC : full_mlayout rows cols)
+  (size_req : prop)
 =
   {| clayout lA |} ->
   {| clayout lB |} ->
@@ -41,7 +48,7 @@ type matmulcomb_gpu_fixed_ty
   stt unit
     (requires
       (cpu ** gA |-> Frac fA eA ** gB |-> Frac fB eB) **
-      (pure (rows * cols <= max_blocks) **
+      (pure size_req **
        gC |-> eC))
     (ensures fun _ ->
       (cpu ** gA |-> Frac fA eA ** gB |-> Frac fB eB) **
@@ -49,7 +56,9 @@ type matmulcomb_gpu_fixed_ty
 
 unfold
 inline_for_extraction
-type matmulcomb_gpu_ty =
+type matmulcomb_gpu_ty
+  (size_req : size_req_t)
+=
   (#et : Type0) -> {| scalar et |} ->
   (comb : binop et) ->
   (#rows : szp) ->
@@ -59,12 +68,15 @@ type matmulcomb_gpu_ty =
   (#lB : full_mlayout shared cols) ->
   (#lC : full_mlayout rows cols) ->
   matmulcomb_gpu_fixed_ty comb lA lB lC
+    (size_req rows shared cols)
 
 (* The type of GPU-side matmuls that only work over already
 tiled matrices. *)
 unfold
 inline_for_extraction
-type tiled_matmulcomb_gpu_ty =
+type tiled_matmulcomb_gpu_ty
+  (size_req : tiled_size_req_t)
+=
   (tile : valid_tile) ->
   (#et : Type0) -> {| scalar et |} ->
   (comb : binop et) ->
@@ -88,8 +100,7 @@ type tiled_matmulcomb_gpu_ty =
   stt unit
     (requires
       (cpu ** gA |-> Frac fA eA ** gB |-> Frac fB eB) **
-      (pure (mrows * mcols <= max_blocks) **
-       pure (tile * tile <= max_threads) **
+      (pure (size_req mrows mshared mcols tile) **
        gC |-> eC))
     (ensures fun _ ->
       (cpu ** gA |-> Frac fA eA ** gB |-> Frac fB eB) **
@@ -159,8 +170,8 @@ type block_tiled1d_matmulcomb_gpu_ty =
     (requires
       (cpu ** gA |-> Frac fA eA ** gB |-> Frac fB eB) **
       (pure (mrows * mcols <= max_blocks) **
-      pure (bm/tm * bn <= max_threads) **
-      gC |-> eC))
+       pure (bm/tm * bn <= max_threads) **
+       gC |-> eC))
     (ensures fun _ ->
       (cpu ** gA |-> Frac fA eA ** gB |-> Frac fB eB) **
       (gC |-> MS.mmcomb comb eC eA eB)
